code/frodo/Hacl.Keccak.fsti
@@ -5,15 +5,19 @@ open Lib.IntTypes
 open Lib.PQ.Buffer
 open Hacl.Impl.PQ.Lib
 
+open LowStar.ModifiesPat
+open LowStar.Modifies
+
+module Buf = LowStar.Buffer
+
 val cshake128_frodo:
   input_len:size_t -> input:lbytes input_len -> cstm:uint16 ->
   output_len:size_t -> output:lbytes output_len -> Stack unit
-  (requires (fun h -> True))
-  (ensures (fun h0 r h1 -> True))
-
+  (requires (fun h -> Buf.live h input /\ Buf.live h output /\ Buf.disjoint input output))
+  (ensures (fun h0 _ h1 -> Buf.live h1 output /\ modifies (loc_buffer output) h0 h1))
 
 val cshake256_frodo:
   input_len:size_t -> input:lbytes input_len -> cstm:uint16 ->
   output_len:size_t -> output:lbytes output_len -> Stack unit
-  (requires (fun h -> True))
-  (ensures (fun h0 r h1 -> True))
+  (requires (fun h -> Buf.live h input /\ Buf.live h output /\ Buf.disjoint input output))
+  (ensures (fun h0 _ h1 -> Buf.live h1 output /\ modifies (loc_buffer output) h0 h1))
